Phi_Semantics/PhiSem_CF_Return.thy
@@ -5,8 +5,11 @@ begin
 section \<open>Semantic\<close>
 
 virtual_datatype \<phi>CF_return_abnormal = \<phi>empty_abnormal +
-  CF_break    :: \<open>VAL list\<close> \<comment> \<open>in unit of bits\<close>
+  ABN_break    :: \<open>VAL list\<close> \<comment> \<open>in unit of bits\<close>
+
 
 print_locale \<phi>CF_return_abnormal
+
+
 
 end
