Phi_System/Calculus_of_Programming.thy
@@ -51,7 +51,7 @@ definition PendingConstruction :: " 'ret proc
                                   \<Rightarrow> resource
                                   \<Rightarrow> assn
                                   \<Rightarrow> ('ret sem \<Rightarrow> assn)
-                                  \<Rightarrow> (ERR sem \<Rightarrow> assn)
+                                  \<Rightarrow> (ABNM sem \<Rightarrow> assn)
                                   \<Rightarrow> bool "
     ("\<^bold>p\<^bold>e\<^bold>n\<^bold>d\<^bold>i\<^bold>n\<^bold>g _ \<^bold>o\<^bold>n _ [_]/ \<^bold>r\<^bold>e\<^bold>s\<^bold>u\<^bold>l\<^bold>t\<^bold>s \<^bold>i\<^bold>n _/ \<^bold>t\<^bold>h\<^bold>r\<^bold>o\<^bold>w\<^bold>s _" [1000,1000,1000,11,11] 10)
     where "PendingConstruction f s R S E \<longleftrightarrow> f s \<subseteq> \<S> (\<lambda>ret. INTERP_SPEC (R * S ret)) (\<lambda>ex. INTERP_SPEC (R * E ex))"
